src/Layers/AbstractLayers/TransactionalDisk/TransactionalDiskLayer.v
@@ -23,7 +23,7 @@ Section TransactionalDisk.
   | Commit : transactional_disk_prog unit
   | Abort : transactional_disk_prog unit
   | Recover : transactional_disk_prog unit
-  | Init : transactional_disk_prog unit.
+  | Init : list addr -> list value -> transactional_disk_prog unit.
 
   Inductive exec' :
     forall T, user -> token' ->  state' -> transactional_disk_prog T -> @Result state' T -> Prop :=
@@ -77,8 +77,8 @@ Section TransactionalDisk.
         exec' u Cont s Recover (Finished (snd s, snd s) tt)
 
   | ExecInit : 
-      forall s u,
-        exec' u Cont s Init (Finished (snd s, snd s) tt)
+      forall s u l_a l_v,
+        exec' u Cont s (Init l_a l_v) (Finished (upd_batch (snd s) l_a l_v, upd_batch (snd s) l_a l_v) tt)
 
   | ExecCrashBefore :
       forall d T (p: transactional_disk_prog T) u,
