src/Refinements/TransactionToTransactionalDisk/Definitions.v
@@ -14,6 +14,7 @@ Definition compile  T (p2: abs_op.(operation) T) : prog imp T.
   exact commit.
   exact abort.
   exact recover.
+  exact init.
 Defined.
 
 Definition token_refines_to  T u (d1: state imp) (p: Core.operation abs_op T) (get_reboot_state: imp.(state) -> imp.(state)) o1 o2 : Prop :=
@@ -98,6 +99,15 @@ Definition token_refines_to  T u (d1: state imp) (p: Core.operation abs_op T) (g
           exec imp u o1 d1 recover (Crashed d1') /\
           o2 = CrashBefore /\
           snd d1' = snd d1)
+      | Init =>
+       (exists d1' r,
+          exec imp u o1 d1 init (Finished d1' r) /\
+          o2 = Cont /\
+          d1' = ([], snd d1)) \/
+       
+       (exists d1',
+          exec imp u o1 d1 init (Crashed d1') /\
+          o2 = CrashBefore)
      end.
 
 Definition refines_to := transaction_rep.
@@ -135,6 +145,15 @@ Definition refines_to_reboot := transaction_reboot_rep.
       unfold refines_to in *; cleanup.
       eapply recover_finished_2 in H0; eauto.
       cleanup; eauto.
+    }
+    {
+      unfold refines_to in *; cleanup.
+      eapply init_finished in H0; eauto.
+      cleanup; eauto.
+      unfold transaction_rep in *; cleanup; eauto.
+      exists (snd x, snd x); repeat cleanup_pairs; eauto.
+      intuition eauto.
+      pose proof (addr_list_to_blocks_length_le []); simpl in *; lia.
     }
   Qed.
 
